



$$
\left[
 \begin{matrix}
   (x-x1)^2+(y-y1)^2 \\
   (x-x2)^2+(y-y2)^2 \\
   (x-x3)^2+(y-y3)^2
  \end{matrix}
  \right] 
  =
  \left[
 \begin{matrix}
   d_1^2 \\
   d_2^2\\
   d_3^2
  \end{matrix}
  \right]
$$

$$
\left[
 \begin{matrix}
   x \\
   y 
  \end{matrix}
  \right]
  =
   \left[
 \begin{matrix}
   2(x1-x3) *  2(y1-y3) \\
   2(x2-x3) *  2(y2-y3) 
  \end{matrix}
  \right] ^{-1}
  \left[
 \begin{matrix}
   x_1^2 -x_3^2+ y_1^2 -y_3^2+d_3^2 -d_1^2\\
   x_1^2 -x_3^2+ y_2^2 -y_3^2+d_3^2 -d_2^2
  \end{matrix}
  \right]
$$

$$
P_r=P_tG_tG_r(\dfrac{\lambda}{4{\pi}d})
$$

$$
P_0=P_tG_tG_r(\dfrac{\lambda}{4{\pi}d_0})
$$

$$
d_0

$$

$$
4{\pi}d^2

$$

$$
3*10^8
$$

$$
\overline{PL}(d)[dB]=\overline{PL}(d)[dB]+10nlog(\dfrac{d}{d_0})
$$

$$
\overline{PL}(d)[dB]=\overline{PL}(d)[dB]+10nlog(\dfrac{d}{d_0})+X_\partial
$$

$$
\partial
$$

